Combinators through repetition

src/parse/Parser.v
@@ -5,317 +5,470 @@ From Pollux.parse Require Import Input.
 From Equations Require Import Equations.
 
 Module Parsers (InputModule : AbstractInput).
-  Import InputModule.
+  Section Parsers.
+    Import InputModule.
 
-  Inductive FailureLevel :=
-  | Fatal
-  | Recoverable.
+    Context `{EqDecision Input}.
 
-  (* Record information about when a parse fails *)
-  Inductive FailureData :=
-  | mkFailureData (msg : string) (remaining : Input) (next : option FailureData).
+    Inductive FailureLevel :=
+    | Fatal
+    | Recoverable.
 
-  Definition getFailureMsg (data : FailureData) : string :=
-    match data with
-    | mkFailureData msg _ _ => msg
-    end.
+    (* Record information about when a parse fails *)
+    Inductive FailureData :=
+    | mkFailureData (msg : string) (remaining : Input) (next : option FailureData).
 
-  Definition getFailureRemaining (data : FailureData) : Input :=
-    match data with
-    | mkFailureData _ remaining _ => remaining
-    end.
+    Definition getFailureMsg (data : FailureData) : string :=
+      match data with
+      | mkFailureData msg _ _ => msg
+      end.
 
-  Definition getFailureNext (data : FailureData) : option FailureData :=
-    match data with
-    | mkFailureData _ _ next => next
-    end.
+    Definition getFailureRemaining (data : FailureData) : Input :=
+      match data with
+      | mkFailureData _ remaining _ => remaining
+      end.
 
-  (* Add more failure data to the end of the current chain of failures *)
-  Fixpoint Concat (self other : FailureData) : FailureData :=
-    match self with
-    | mkFailureData msg remaining next =>
-        match next with
-        | None => mkFailureData msg remaining (Some other)
-        | Some next_val => mkFailureData msg remaining (Some (Concat next_val other))
-        end
-    end.
-  
-  Inductive ParseResult {R : Type} :=
-  | ParseSuccess (result : R) (remaining : Input)
-  | ParseFailure (level : FailureLevel) (data : FailureData).
-  
-  Arguments ParseResult R : clear implicits.
+    Definition getFailureNext (data : FailureData) : option FailureData :=
+      match data with
+      | mkFailureData _ _ next => next
+      end.
 
-  (**
+    (* Add more failure data to the end of the current chain of failures *)
+    Fixpoint ConcatFailure (self other : FailureData) : FailureData :=
+      match self with
+      | mkFailureData msg remaining next =>
+          match next with
+          | None => mkFailureData msg remaining (Some other)
+          | Some next_val => mkFailureData msg remaining (Some (ConcatFailure next_val other))
+          end
+      end.
+    
+    Inductive ParseResult {R : Type} :=
+    | ParseSuccess (result : R) (remaining : Input)
+    | ParseFailure (level : FailureLevel) (data : FailureData).
+    
+    Arguments ParseResult R : clear implicits.
+
+    (**
      FUNCTIONS ON PARSE RESULTS
-   *)
+     *)
 
-  (* If Remaining is the same as the input, then parser is "uncommitted",
+    (* If Remaining is the same as the input, then parser is "uncommitted",
      so combinators like Or or ZeroOrMore can try alternatives. *)
-  Definition Remaining {R : Type} (pr : ParseResult R) : Input :=
-    match pr with
-    | ParseSuccess _ rem
-    | ParseFailure _ (mkFailureData _ rem _) => rem
-    end.
-  
-  Definition IsFailure {R : Type} (pr : ParseResult R) : bool :=
-    match pr with
-    | ParseFailure _ _ => true
-    | _ => false
-    end.
+    Definition Remaining {R : Type} (pr : ParseResult R) : Input :=
+      match pr with
+      | ParseSuccess _ rem
+      | ParseFailure _ (mkFailureData _ rem _) => rem
+      end.
+    
+    Definition IsFailure {R : Type} (pr : ParseResult R) : bool :=
+      match pr with
+      | ParseFailure _ _ => true
+      | _ => false
+      end.
 
-  Definition IsFatalFailure {R : Type} (pr : ParseResult R) : bool :=
-    match pr with
-    | ParseFailure Fatal _ => true
-    | _ => false
-    end.
+    Definition IsFatalFailure {R : Type} (pr : ParseResult R) : bool :=
+      match pr with
+      | ParseFailure Fatal _ => true
+      | _ => false
+      end.
 
-  Definition IsFailureProp {R : Type} (pr : ParseResult R) : Prop :=
-    match pr with
-    | ParseSuccess _ _ => False
-    | ParseFailure _ _ => True
-    end.
+    Definition IsFailureProp {R : Type} (pr : ParseResult R) : Prop :=
+      match pr with
+      | ParseSuccess _ _ => False
+      | ParseFailure _ _ => True
+      end.
 
-  (* This function basically lets us change the parameterized type of a parse failure. This is useful
+    (* This function basically lets us change the parameterized type of a parse failure. This is useful
      if we imagine that parsing a number depends are first parsing a list of digits. If we fail to
      parse the list of digits, we want to propagate that error up as the result of paring the number
      but can't (directly) do this since the type of the failure is wrong. This function constructs
      the same parse failure but with the correct type. It takes a proof term as input since this
      only makes sense for failures. Successes with have something of type R in them, which we can't
      convert to a U. *)
-  Definition PropagateFailure {R : Type} {U : Type} (pr : ParseResult R) (pf : IsFailureProp pr) :
-    ParseResult U.
-  Proof.
-    destruct pr.
-    - destruct pf.
-    - apply ParseFailure; assumption.
-  Defined.
+    Definition PropagateFailure {R : Type} {U : Type} (pr : ParseResult R) (pf : IsFailureProp pr) :
+      ParseResult U.
+    Proof.
+      destruct pr.
+      - destruct pf.
+      - apply ParseFailure; assumption.
+    Defined.
 
-  (* Similarly to PropagateFailure, this function only works on a ParseSuccess and lets us unwrap it.
+    (* Similarly to PropagateFailure, this function only works on a ParseSuccess and lets us unwrap it.
      Honestly, both of these could be done inline whenever needed, but I like learning more about how
      to handle these in Rocq. I don't know what extraction would do to these. *)
-  Definition IsSuccessProp {R : Type} (pr : ParseResult R) : Prop :=
-    match pr with
-    | ParseSuccess _ _ => True
-    | ParseFailure _ _ => False
-    end.
+    Definition IsSuccessProp {R : Type} (pr : ParseResult R) : Prop :=
+      match pr with
+      | ParseSuccess _ _ => True
+      | ParseFailure _ _ => False
+      end.
 
-  Definition Extract {R : Type} (pr : ParseResult R) (pf : IsSuccessProp pr) : R * Input. 
-  Proof.
-    destruct pr.
-    - split; assumption.
-    - destruct pf.
-  Defined.
+    Definition Extract {R : Type} (pr : ParseResult R) (pf : IsSuccessProp pr) : R * Input. 
+    Proof.
+      destruct pr.
+      - split; assumption.
+      - destruct pf.
+    Defined.
 
-  Definition ResultMap {R : Type} {R' : Type} (pr : ParseResult R) (f : R -> R') : ParseResult R' :=
-    match pr with
-    | ParseSuccess result remaining => ParseSuccess (f result) remaining
-    | ParseFailure lvl data => ParseFailure lvl data
-    end.
+    Definition ResultMap {R : Type} {R' : Type} (pr : ParseResult R) (f : R -> R') : ParseResult R' :=
+      match pr with
+      | ParseSuccess result remaining => ParseSuccess (f result) remaining
+      | ParseFailure lvl data => ParseFailure lvl data
+      end.
 
-  Definition MapRecoverableError {R : Type} (pr : ParseResult R) (f : FailureData -> FailureData) :
-    ParseResult R :=
-    match pr with
-    | ParseFailure Recoverable data => ParseFailure Recoverable (f data)
-    | _ => pr
-    end.
+    Definition MapRecoverableError {R : Type} (pr : ParseResult R) (f : FailureData -> FailureData) :
+      ParseResult R :=
+      match pr with
+      | ParseFailure Recoverable data => ParseFailure Recoverable (f data)
+      | _ => pr
+      end.
 
-  Definition NeedsAlternative {R : Type} `{EqDecision Input} (pr : ParseResult R) (input : Input) : bool :=
-    match pr with
-    | ParseFailure Recoverable (mkFailureData _ rem _) => if rem == input then true else false
-    | _ => false
-    end.
+    Definition NeedsAlternative {R : Type} (pr : ParseResult R) (input : Input) : bool :=
+      match pr with
+      | ParseFailure Recoverable (mkFailureData _ rem _) => if rem == input then true else false
+      | _ => false
+      end.
 
-  (**
+    (**
      Parser Definition
 
      This are missing Dafny variance specifiers. I don't know how big of a problem this will be
-  *)
+     *)
 
-  (* A parser is a total function from a position to a parse result *)
-  Definition Parser {R : Type} := Input -> ParseResult R.
-  Arguments Parser R : clear implicits.
+    (* A parser is a total function from a position to a parse result *)
+    Definition Parser {R : Type} := Input -> ParseResult R.
+    Arguments Parser R : clear implicits.
 
-  (* A parser selector is a function that, given a name that exists,
+    (* A parser selector is a function that, given a name that exists,
      returns a parser associated to this name *)
-  Definition ParserSelector {R : Type} := string -> ParseResult R.
-  Arguments ParserSelector R : clear implicits.
+    Definition ParserSelector {R : Type} := string -> ParseResult R.
+    Arguments ParserSelector R : clear implicits.
 
-  (**
+    (**
      Misc Utilities and Definitions
-   *)
-  Definition IsRemaining (input remaining : Input) : Prop :=
-    Length remaining <= Length input /\ Drop input (Length input - Length remaining) = remaining.
+     *)
+    Definition IsRemaining (input remaining : Input) : Prop :=
+      Length remaining <= Length input /\ Drop input (Length input - Length remaining) = remaining.
 
-  Lemma IsRemainingTrans (input remaining1 remaining2 : Input) :
-    IsRemaining input remaining1 -> IsRemaining remaining1 remaining2 -> IsRemaining input remaining2.
-  Proof.
-    intros [H1_len H1_drop] [H2_len H2_drop].
-    unfold IsRemaining.
-    split.
-    - apply Nat.le_trans with (Length remaining1); assumption.
-    - rewrite <- H2_drop at 2. 
-      rewrite <- H1_drop at 1.
-      rewrite <- DropDrop.
-      * rewrite Nat.add_sub_assoc; last assumption.
-        rewrite Nat.sub_add; last assumption.
-        reflexivity.
-      * lia.
-      * lia.
-  Qed.
+    Lemma IsRemainingTrans (input remaining1 remaining2 : Input) :
+      IsRemaining input remaining1 -> IsRemaining remaining1 remaining2 -> IsRemaining input remaining2.
+    Proof.
+      intros [H1_len H1_drop] [H2_len H2_drop].
+      unfold IsRemaining.
+      split.
+      - apply Nat.le_trans with (Length remaining1); assumption.
+      - rewrite <- H2_drop at 2. 
+        rewrite <- H1_drop at 1.
+        rewrite <- DropDrop.
+        * rewrite Nat.add_sub_assoc; last assumption.
+          rewrite Nat.sub_add; last assumption.
+          reflexivity.
+        * lia.
+        * lia.
+    Qed.
 
-  (**
+    (**
      COMBINATORS
-  *)
-  (* This parser does not consume any input and returns the given value *)
-  Definition SucceedWith {R : Type} (result : R) : Parser R :=
-    (fun inp => ParseSuccess result inp).
+     *)
+    (* This parser does not consume any input and returns the given value *)
+    Definition SucceedWith {R : Type} (result : R) : Parser R :=
+      (fun inp => ParseSuccess result inp).
 
-  (* A parser that always succeeds, consumes nothing and returns () *)
-  Definition Epsilon : (Parser unit) := SucceedWith ().
+    (* A parser that always succeeds, consumes nothing and returns () *)
+    Definition Epsilon : (Parser unit) := SucceedWith ().
 
-  (* A parser that does not consume any input and returns the given failure *)
-  Definition FailWith {R : Type} (message : string) (level : FailureLevel) : Parser R :=
-    (fun inp => ParseFailure level $ mkFailureData message inp None).
+    (* A parser that does not consume any input and returns the given failure *)
+    Definition FailWith {R : Type} (message : string) (level : FailureLevel) : Parser R :=
+      (fun inp => ParseFailure level $ mkFailureData message inp None).
 
-  (* A parser that always returns the given result *)
-  Definition ResultWith {R : Type} (result : ParseResult R) : Parser R :=
-    (fun inp => result).
+    (* A parser that always returns the given result *)
+    Definition ResultWith {R : Type} (result : ParseResult R) : Parser R :=
+      (fun inp => result).
 
-  (* A parser that fails if the string has not been entirely consumed *)
-  Definition EndOfString : Parser unit :=
-    (fun inp => if Length inp == 0 then
-               ParseSuccess () inp
-             else
-               ParseFailure Recoverable
-                 (mkFailureData "expected end of string" inp None)).
+    (* A parser that fails if the string has not been entirely consumed *)
+    Definition EndOfString : Parser unit :=
+      (fun inp => if Length inp == 0 then
+                 ParseSuccess () inp
+               else
+                 ParseFailure Recoverable
+                   (mkFailureData "expected end of string" inp None)).
 
-  (* A parser that fails if the left parser fails. If the left parser succeeds, provides its
+    (* A parser that fails if the left parser fails. If the left parser succeeds, provides its
      result and the remaining sequence to the right parser generator. *)
-  Definition Bind {L R : Type} (left : Parser L) (right : L -> Parser R) : Parser R :=
-    fun inp =>
-      match left inp with
-      | ParseSuccess leftResult remaining => right leftResult remaining
-      | ParseFailure level data => ParseFailure level data
-      end.
+    Definition Bind {L R : Type} (left : Parser L) (right : L -> Parser R) : Parser R :=
+      fun inp =>
+        match left inp with
+        | ParseSuccess leftResult remaining => right leftResult remaining
+        | ParseFailure level data => ParseFailure level data
+        end.
 
-  (* A parser that fails if the left parser fails. If the left parser succeeds, provides its
+    (* A parser that fails if the left parser fails. If the left parser succeeds, provides its
      result to the right parser generator and returns its result applied to the remaining input *)
-  Definition BindSucceeds {L R : Type} (left : Parser L) (right : L -> Input -> Parser R) : Parser R :=
-    fun inp =>
-      match left inp with
-      | ParseSuccess leftResult remaining => right leftResult remaining remaining
-      | ParseFailure level data => ParseFailure level data
-      end.
+    Definition BindSucceeds {L R : Type} (left : Parser L) (right : L -> Input -> Parser R) : Parser R :=
+      fun inp =>
+        match left inp with
+        | ParseSuccess leftResult remaining => right leftResult remaining remaining
+        | ParseFailure level data => ParseFailure level data
+        end.
 
-  (* Given a left parser and a parser generator based on the output of the left parser,
+    (* Given a left parser and a parser generator based on the output of the left parser,
      returns the result of the right parser applied on the original input. *)
-  Definition BindResult {L R : Type} (left : Parser L) (right : ParseResult L -> Input -> Parser R) : Parser R :=
-    fun inp =>
-      right (left inp) inp inp.
+    Definition BindResult {L R : Type} (left : Parser L) (right : ParseResult L -> Input -> Parser R) : Parser R :=
+      fun inp =>
+        right (left inp) inp inp.
 
-  Definition Map {R U : Type} (underlying : Parser R) (f : R -> U) : Parser U :=
-    fun inp =>
-      match underlying inp with
-      | ParseSuccess leftResult remaining => ParseSuccess (f leftResult) remaining
-      | ParseFailure level data => ParseFailure level data
-      end.
+    Definition Map {R U : Type} (underlying : Parser R) (f : R -> U) : Parser U :=
+      fun inp =>
+        match underlying inp with
+        | ParseSuccess leftResult remaining => ParseSuccess (f leftResult) remaining
+        | ParseFailure level data => ParseFailure level data
+        end.
 
-  (* Returns a parser that succeeds if the underlying parser fails and vice-versa.
+    (* Returns a parser that succeeds if the underlying parser fails and vice-versa.
      The result does not consume any input. *)
-  Definition Not {R : Type} (underlying : Parser R) : Parser unit :=
-    fun inp =>
-      match underlying inp with
-      | ParseFailure level data as result =>
-          if IsFatalFailure result then
-            PropagateFailure result I
-          else
-            ParseSuccess () inp
-      | ParseSuccess _ _ => ParseFailure Recoverable (mkFailureData "not failed" inp None)
-      end.
+    Definition Not {R : Type} (underlying : Parser R) : Parser unit :=
+      fun inp =>
+        match underlying inp with
+        | ParseFailure level data as result =>
+            if IsFatalFailure result then
+              PropagateFailure result I
+            else
+              ParseSuccess () inp
+        | ParseSuccess _ _ => ParseFailure Recoverable (mkFailureData "not failed" inp None)
+        end.
 
-  (* Make the two parsers parse the same string and, if both succeed, return a pair of the
+    (* Make the two parsers parse the same string and, if both succeed, return a pair of the
      two results, with the remaining of the right parser.
 
      If one parser fails, return that parse failure. If both fail, return the left failure
-   *)
-  Definition And {L R : Type} (left : Parser L) (right : Parser R) : Parser (L * R) :=
-    fun inp =>
-      match left inp, right inp with
-      | ParseSuccess l _, ParseSuccess r rr => ParseSuccess (l, r) rr
-      | ParseFailure level data, _
-      | _, ParseFailure level data => ParseFailure level data
+     *)
+    Definition And {L R : Type} (left : Parser L) (right : Parser R) : Parser (L * R) :=
+      fun inp =>
+        match left inp, right inp with
+        | ParseSuccess l _, ParseSuccess r rr => ParseSuccess (l, r) rr
+        | ParseFailure level data, _
+        | _, ParseFailure level data => ParseFailure level data
+        end.
+
+    Definition Or {R : Type} (left : Parser R) (right : Parser R) : Parser R :=
+      fun inp =>
+        match left inp with
+        | ParseSuccess r rem as p => p
+        | ParseFailure _ data as p =>
+            if negb $ NeedsAlternative p inp then
+              p
+            else 
+              let p2 := right inp in
+              if negb $ NeedsAlternative p2 inp then
+                p2
+              else
+                MapRecoverableError p2 (fun dataRight => ConcatFailure data dataRight)
+        end.
+
+    (* Like Or, but takes as many parsers as needed *)
+    Fixpoint OrSeq {R : Type} (alternatives : list (Parser R)) : Parser R :=
+      match alternatives with
+      | [] => FailWith "no alternatives" Recoverable
+      | alt :: [] => alt
+      | alt :: alts => Or alt (OrSeq alts)
       end.
 
-  Definition Or {R : Type} `{EqDecision Input} (left : Parser R) (right : Parser R) : Parser R :=
-    fun inp =>
-      match left inp with
-      | ParseSuccess r rem as p => p
-      | ParseFailure _ data as p =>
-          if negb $ NeedsAlternative p inp then
-            p
-          else 
-            let p2 := right inp in
-            if negb $ NeedsAlternative p2 inp then
-              p2
-            else
-              MapRecoverableError p2 (fun dataRight => Concat data dataRight)
-      end.
-
-  (* Like Or, but takes as many parsers as needed *)
-  Fixpoint OrSeq {R : Type} `{EqDecision Input} (alternatives : list (Parser R)) : Parser R :=
-    match alternatives with
-    | [] => FailWith "no alternatives" Recoverable
-    | alt :: [] => alt
-    | alt :: alts => Or alt (OrSeq alts)
-    end.
-
-  (* If the underlying parser succeeds, return it's result without committing the input.
+    (* If the underlying parser succeeds, return it's result without committing the input.
      If the underlying parser fails,
      - with a fatal failure, return it as-is
      - with a recoverable failure, return it without committing the input *)
-  Definition Lookahead {R : Type} (underlying : Parser R) : Parser R :=
-    fun inp =>
-      match underlying inp with
-      | ParseSuccess r rem => ParseSuccess r inp
-      | ParseFailure Fatal data as p => p
-      | ParseFailure Recoverable data => ParseFailure Recoverable (mkFailureData (getFailureMsg data) inp None)
-      end.
+    Definition Lookahead {R : Type} (underlying : Parser R) : Parser R :=
+      fun inp =>
+        match underlying inp with
+        | ParseSuccess r rem => ParseSuccess r inp
+        | ParseFailure Fatal data as p => p
+        | ParseFailure Recoverable data => ParseFailure Recoverable (mkFailureData (getFailureMsg data) inp None)
+        end.
 
-  (* (Opt a) evaluates `a` on the input, and then
+    (* (Opt a) evaluates `a` on the input, and then
      - If `a` succeeds, return the result unchanged
      - If `a` fails, and the failure is not fatal, propagate the same failure without consuming input.
 
      (Opt a) is useful when there are alternatives to parse and `a` parsed partially and we're OK with
      backtracking to try something else. *)
-  Definition Opt {R : Type} (underlying : Parser R) : Parser R :=
-    fun inp =>
-      match underlying inp with
-      | ParseSuccess r rem as p => p
-      | ParseFailure Fatal data as p => p
-      | ParseFailure Recoverable data => ParseFailure Recoverable (mkFailureData (getFailureMsg data) inp None)
-      end.
-                                         
-  (* If the condition parser fails, returns a non-committing failure.
+    Definition Opt {R : Type} (underlying : Parser R) : Parser R :=
+      fun inp =>
+        match underlying inp with
+        | ParseSuccess r rem as p => p
+        | ParseFailure Fatal data as p => p
+        | ParseFailure Recoverable data => ParseFailure Recoverable (mkFailureData (getFailureMsg data) inp None)
+        end.
+    
+    (* If the condition parser fails, returns a non-committing failure.
      Suitable to use in Or parsers. *)
-  Definition If {L R : Type} (condition : Parser L) (succeed : Parser R) : Parser R :=
-    Bind (Lookahead condition) (fun _ => succeed).
-  
-  (* (Maybe a) evaluates `a` on the input, and then
+    Definition If {L R : Type} (condition : Parser L) (succeed : Parser R) : Parser R :=
+      Bind (Lookahead condition) (fun _ => succeed).
+    
+    (* (Maybe a) evaluates `a` on the input, and then
      - If `a` succeeds, wraps the result in Some
      - If `a` fails, and the failure is not fatal and did not consume input, succeeds with None.
        If the error is fatal or did consume input, fails with the same failure. *)
-  Definition Maybe {R : Type} `{EqDecision Input} (underlying : Parser R) : Parser (option R) :=
-    fun inp =>
+    Definition Maybe {R : Type} (underlying : Parser R) : Parser (option R) :=
+      fun inp =>
+        match underlying inp with
+        | ParseSuccess rr rem => ParseSuccess (Some rr) rem
+        | ParseFailure Fatal data as pr => PropagateFailure pr I
+        | ParseFailure Recoverable data as pr => if negb $ NeedsAlternative pr inp then
+                                                  PropagateFailure pr I
+                                                else
+                                                  ParseSuccess None inp
+        end.
+
+    (* Apply two consecutive parsers consecutively. If both succeed, apply the mapper to the result
+     and return it *)
+    Definition ConcatMap {L R T : Type} (left : Parser L) (right : Parser R) (mapper : L -> R -> T) : Parser T :=
+      fun inp =>
+        match left inp with
+        | ParseSuccess ll lrem => match right lrem with
+                                 | ParseSuccess rr rrem => ParseSuccess (mapper ll rr) rrem
+                                 | ParseFailure lvl data as p => PropagateFailure p I
+                                 end
+        | ParseFailure lvl data as p => PropagateFailure p I
+        end.
+
+    (* Apply two parser consecutively. If both succeed, return the pair of both results *)
+    Definition Concat {L R : Type} (left : Parser L) (right : Parser R) : Parser (L * R) :=
+      fun inp =>
+        match left inp with
+        | ParseSuccess ll lrem => match right lrem with
+                                 | ParseSuccess rr rrem => ParseSuccess (ll, rr) rrem
+                                 | ParseFailure lvl data as p => PropagateFailure p I
+                                 end
+        | ParseFailure lvl data as p => PropagateFailure p I
+        end.
+
+    (* Return only the result of the right parser if the two parsers match *)
+    Definition ConcatKeepRight {L R : Type} (left : Parser L) (right : Parser R) : Parser R :=
+      ConcatMap left right (fun l r => r).
+    
+    (* Return only the result of the left parser if the two parsers match *)
+    Definition ConcatKeepLeft {L R : Type} (left : Parser L) (right : Parser R) : Parser L :=
+      ConcatMap left right (fun l r => l).
+    
+    (* TODO debug parser? Might just need to be in OCaml since Rocq I/O functions seem funky *)
+
+    Definition rep'_memory {A : Type} (underlying : Parser A) (inp : Input) : (ParseResult A * bool) :=
       match underlying inp with
-      | ParseSuccess rr rem => ParseSuccess (Some rr) rem
-      | ParseFailure Fatal data as pr => PropagateFailure pr I
-      | ParseFailure Recoverable data as pr => if negb $ NeedsAlternative pr inp then
-                                                PropagateFailure pr I
-                                              else
-                                                ParseSuccess None inp
+      | ParseSuccess ret rem as p => if Nat.ltb (Length rem) (Length inp) then
+                                      (p, true)
+                                    else
+                                      (p, false)
+      | ParseFailure lvl data as p => (p, true)
       end.
-  
+
+    Lemma rep'_memory_len {A : Type} (underlying : Parser A) (inp : Input) :
+      forall ret rem,
+      rep'_memory underlying inp = (ParseSuccess ret rem, true) -> Length rem < Length inp.
+    Proof.
+      intros ret rem.
+      unfold rep'_memory.
+      destruct (underlying inp) eqn:Hp.
+      - destruct (Length remaining <? Length inp) eqn:Hn.
+        * destruct (Nat.ltb_spec (Length remaining) (Length inp)) in Hn.
+        + intros Hinv. inversion Hinv. subst. assumption.
+        + discriminate.
+          * intros Hinv. inversion Hinv.
+      - intros Hinv. inversion Hinv.
+    Qed.
+
+    (* The primitive repetition combinator which applies the underlying parser over the input
+     until a recoverable failure happens and returns the accumulated results *)
+    (* Defined below, Rep' is the repetition primitive in the parser combinators for Dafny.
+     In this version, we use well-founded recursion to ensure it terminates.
+     In order to the equations plugin to record the decision of the if statement, I'm using
+     decide here, which enables near automatic handling of this fact.
+
+     However, this leads to warnings:
+
+     Warning:
+     The decreasing recursive call obligation Rep'_obligation_2 could not be defined as a hint:
+     Rep'_obligation_2 cannot be used as a hint. [wf-obligation-cannot-be-used,equations,default]
+     Warning:
+     The decreasing recursive call obligation Rep'_obligation_3 could not be defined as a hint:
+     Rep'_obligation_3 cannot be used as a hint. [wf-obligation-cannot-be-used,equations,default]
+
+     I tried to rewrite this to not use `decide`, which resulted in rep'_memory above. The idea
+     there was that since I can use `inspect` and the eqn:H notation to record facts for obligation proofs,
+     the helper function would let me inject the fact that Nat.ltb (Length rem) (Length inp) is true into
+     the obligation context, which I could then solve easily. Unfortunately, this led to the same warnings
+     being issued, so for the moment I've reverted to the self-contained version using decide.
+     *)
+    Equations? Rep' {A B : Type} (underlying : Parser B) (combine : A -> B -> A) (acc : A)
+      (inp : Input) : ParseResult A by wf (Length inp) lt :=
+      Rep' underlying combine acc inp with underlying inp => {
+        | ParseSuccess ret rem => if decide (Length rem < Length inp) then
+                                   Rep' underlying combine (combine acc ret) rem
+                                 else
+                                   ParseSuccess acc inp
+        | ParseFailure lvl data => if NeedsAlternative (ParseFailure lvl data) inp then
+                                    ParseSuccess acc inp
+                                  else
+                                    PropagateFailure (ParseFailure lvl data) I
+        }.
+    Proof.
+      all: try done.
+    Qed.
+
+    (* Proof for the memory version *)
+    (*   apply rep'_memory_len in H. *)
+    (*   assumption. *)
+    (* Qed. *)
+
+    (* Repeats the underlying parser until the first failure that accepts alternatives, combining results
+     into an accumulator and return the final accumulated result. *)
+    Definition Rep {A B : Type} (underlying : Parser B) (combine : A -> B -> A) (acc : A) :
+      Parser A :=
+      fun inp => Rep' underlying combine acc inp.
+
+    (* Repeats the underlying parser interleaved with a separator. Returns a sequence of results *)
+    Definition RepSep {A B : Type} (underlying : Parser A) (separator : Parser B) :
+      Parser (list A) :=
+      Bind (Maybe underlying)
+        (fun (result : option A) =>
+           match result with
+           | Some ret => Rep (ConcatKeepRight separator underlying)
+                          (fun (acc : list A) (a : A) => acc ++ [a])
+                          ([ret])
+           | None => SucceedWith []
+           end).
+
+    (* Repeats the underlying parser, merging intermediate results. Returns the final merged result. *)
+    Definition RepMerge {A : Type} (underlying : Parser A) (merger : A -> A -> A) : Parser A :=
+      Bind (Maybe underlying)
+        (fun (result : option A) =>
+           match result with
+           | Some ret => Rep underlying merger ret
+           | None => FailWith "No first element in RepMerge" Recoverable
+           end).
+
+    (* Repeats the underlying parser separated by the given separator parser, merging intermediate results.
+     Returns the final merged result. *)
+    Definition RepSepMerge {A B : Type} (underlying : Parser A) (separator : Parser B)
+      (merger : A -> A -> A) : Parser A :=
+      Bind (Maybe underlying)
+        (fun (result : option A) =>
+           match result with
+           | Some ret => Rep (ConcatKeepRight separator underlying) merger ret
+           | None => FailWith "No first element in RepSepMerge" Recoverable
+           end).
+
+    (* Repeated the underlying parser until the first failure that accepts alternatives, and returns the
+       underlying sequence. *)
+    Definition ZeroOrMore {R : Type} (underlying : Parser R) : Parser (list R) :=
+      Rep underlying (fun (acc : list R) (r : R) => acc ++ [r]) [].
+
+    (* Like ZeroOrMore but will return a failure if there is not at least one match. *)
+    Definition OneOrMore {R : Type} (underlying : Parser R) : Parser (list R) :=
+      Bind underlying
+        (fun r =>
+           Rep underlying (fun (acc : list R) (r : R) => acc ++ [r]) [r]).
+
+  End Parsers.
 End Parsers.
 
 Module test.
@@ -325,7 +478,7 @@ Module test.
 
   Compute IsFatalFailure (ParseFailure Recoverable (mkFailureData "" [] None)).
   Compute let pr := ParseFailure Recoverable (mkFailureData "" [] None) in
-            PropagateFailure pr I : ParseResult bool.
+            PropagateFailure pr I : @ParseResult bool.
   Compute let pr := ParseSuccess 10 [] in
             Extract pr I.
 
